#heapsort #algorithm #time-complexity #Algorithm-4th
### Time Complexity of the Heapsort Algorithm

The time complexity of the heapsort algorithm, $T(n) = O(n \log n)$.
- The `heapify` function takes $O(\log n)$.
- The `build-max/min-heap` function takes $O(n)$.
- Since every node needs to perform `heapify`, and for each `heapify`, it will perform at most $h$ (the height of the complete binary tree, which equals $\log_2 n$) swaps, the time complexity will be $O(n \log n)$.

### The difference between heap and priority queue

A priority queue is an abstract data type (ADT) that defines the behavior of managing data. It can be implemented in various ways, including using a heap.

### Calculation of indices

1. Assume the index of the root is 0, the left child is 1, and the right child is 2. Initially, we might think that `index(left) = index(parent) + 1` and `index(right) = index(parent) + 2`.
2. However, when it comes to the first left child (index = 1), its `leftChild = 3` and `rightChild = 4`. So, we need to update our calculation. The final calculation will be:
   1. `index(left) = 2 * index(parent) + 1`
   2. `index(right) = 2 * index(parent) + 2`
3. To find the index of the parent, we can use the following formula: `index(parent) = floor((index(child) - 1) / 2)`


### The recurrence of $T(n) = T\left(\frac{2n}{3}\right) + O(1)$:

1. Assume, in the worst case, for height $h \geq 1$, the tree has $2^{h-1}$ leaves on its last level. That is, the left child of the root is a perfect binary tree, while the right child is also a perfect binary tree but has $2^{h-1}$ fewer nodes compared to the left child of the root.
2. Given an example:
   1. Left: $1 + 2 + 4 + 8 + 16$
   2. Right: $1 + 2 + 4 + 8$
3. Generalizing this, we get:
   1. Left: $2^0 + 2^1 + 2^2 + 2^3 + 2^4$
   2. Right: $2^0 + 2^1 + 2^2 + 2^3$
4. To further generalize, let‚Äôs say we have $h = 5$:
   1. Left: $2^0 + 2^1 + \cdots + 2^{h-1}$
   2. Right: $2^0 + 2^1 + \cdots + 2^{h-2}$
5. Using the summation of a geometric progression, we have:
   1. $\text{Left} = \frac{a(r^n - 1)}{r - 1} = \frac{1 \cdot (2^{h-1+1} - 1)}{2 - 1} = 2^h - 1$ (since $2^0$ is also one of the elements)
   2. $\text{Right} = \frac{a(r^n - 1)}{r - 1} = \frac{1 \cdot (2^{h-2+1} - 1)}{2 - 1} = 2^{h-1} - 1$
6. So, in the most unbalanced case:
$$\frac{\text{Left}}{\text{Total}} = \frac{2^h - 1}{(2^h - 1) + (2^{h-1} - 1) + 1}$$
$$\frac{\text{Left}}{\text{Total}} = \frac{2(2^{h-1}) - 1}{2(2^{h-1}) + 2^{h-1} - 1}$$
$$\frac{\text{Left}}{\text{Total}} = \frac{2(2^{h-1}) - 1}{3(2^{h-1}) - 1}$$
    As $h \rightarrow \infty$,
$$
\lim_{h \to \infty} \frac{2(2^{h-1})}{3(2^{h-1})} = \frac{2}{3}
$$


### Implementation


### Reference
---
 1. [How is the reccurence of Max Heapify T(n)= T(2n/3) +¬†Œ∏(1)ùúÉ(1)?](https://cs.stackexchange.com/questions/141748/how-is-the-reccurence-of-max-heapify-tn-t2n-3-theta1)
 2. [Worst case in Max-Heapify - How do you get 2n/3?](https://stackoverflow.com/questions/9099110/worst-case-in-max-heapify-how-do-you-get-2n-3)